stick all invariants in lock invariant

src/Examples/DistributedCtr/DistCtrImpl_Local.v
@@ -23,43 +23,32 @@ Definition kill_node: val :=
 
 Section proof.
   Context `{!heapG Σ, !spawnG Σ, !lockG Σ, !inG Σ (authR (optionUR (exclR ZO)))}.
-  Definition nodeN : namespace := nroot .@ "node".
-
-  Definition node_val_prop (node: loc) (isDead: Prop) (γ : gname): iProp Σ :=
-    ∃ (n: Z), ((⌜isDead⌝ ∧ node ↦ NONEV) ∨ (⌜~isDead⌝ ∧ node ↦ SOMEV #n))%I.
 
   Definition node_own_inv (node: loc) (n : Z) (γ : gname): iProp Σ :=
     own γ (◯ (Excl' n))%I.
 
-  Definition node_val_inv (node: loc) (isDead: Prop) (γ : gname): iProp Σ :=
-    inv nodeN (node_val_prop node isDead γ)%I.
-
-  Definition node_lock_inv (γ: gname) : iProp Σ :=
-    (∃ n, own γ (● (Excl' n)))%I.
+  Definition node_lock_inv (node: loc) (isDead: Prop) (γ: gname) : iProp Σ :=
+    (∃ n, own γ (● (Excl' n))
+    ∗ ((⌜isDead⌝ ∧ node ↦ NONEV) ∨ (⌜~isDead⌝ ∧ node ↦ SOMEV #n)))%I.
 
   Lemma alloc_node_spec : 
     {{{ True%I }}}
       alloc_node #()
-      {{{ r1 lk γ γ1, RET PairV #r1 lk;
-          is_lock LockN γ lk (node_lock_inv γ1)
-          ∗ node_val_inv r1 false γ1
-          ∗ node_own_inv r1 0 γ1
+      {{{ node lk γ γ1, RET PairV #node lk;
+          is_lock LockN γ lk (node_lock_inv node false γ1)
     }}}.
   Proof.
     iIntros (Φ) "_ HPost".
     iMod (ghost_var_alloc 0) as (γ1) "[Hγ1● Hγ1◯]".
 
     unfold alloc_node.
-    wp_alloc master as "Hr1".
+    wp_alloc node as "Hr1".
     wp_let.
  
-    wp_apply (newlock_spec LockN (node_lock_inv γ1) with "[- Hγ1◯ Hr1 HPost]").
-    iExists 0; auto.
+    wp_apply (newlock_spec LockN (node_lock_inv node false γ1) with "[- Hγ1◯ HPost]").
+    iExists 0. iFrame. iRight;auto.
     iIntros (lk γ) "HIsLk".
     wp_let.
-    iMod (inv_alloc nodeN _ (node_val_prop master false γ1) with "[Hr1]") as "#Hinv".
-    { unfold node_val_prop. iNext. iExists 0. iRight; iSplit; auto. }
-
     wp_pures.
     iApply "HPost".
     iFrame; auto.
@@ -67,91 +56,58 @@ Section proof.
 
   Lemma update_node_some_spec : ∀ (n: Z) γ1 node,
       {{{
-           node_lock_inv γ1
-          ∗ node_val_inv node false γ1
+           node_lock_inv node false γ1
           ∗ node_own_inv node n γ1
     }}}
       update_node #node
     {{{ RET #1;
-          node_lock_inv γ1
-          ∗ node_val_inv node false γ1
+          node_lock_inv node false γ1
           ∗ node_own_inv node (n+1) γ1
     }}}.
   Proof.
-    iIntros (n γ1 node Φ) "(Hlkinv & #Hnodeinv & Hγ1◯) HPost".
-    unfold node_val_inv.
-    unfold node_val_prop.
-    unfold update_node.
+    iIntros (n γ1 node Φ) "(Hlkinv & Hγ1◯) HPost".
     unfold node_lock_inv.
     unfold node_own_inv.
+    unfold update_node.
     wp_pures.
 
-    wp_bind ( ! #node )%E.
-    iInv "Hnodeinv" as ">Hinv".
-    iDestruct "Hinv" as (n') "[[H Halive] | [H Halive]]";
+    iDestruct "Hlkinv" as (n') "(Hγ1● & [[H Halive] | [H Halive]])";
     wp_load;
-    iDestruct "H" as %H. inversion H.
-    iModIntro.
-    iSplitL "Halive".
-    { iNext. unfold node_val_prop. iExists n'. iRight. iSplitR "Halive"; auto. }
-
+    iDestruct "H" as %H. inversion H; subst.
     wp_pures.
-    wp_bind ( #node <- _ )%E.
-    iInv "Hnodeinv" as ">Hinv".
-    iDestruct "Hinv" as (n0) "[[H Halive] | [H Halive]]";
-    iDestruct "H" as %H'. inversion H'.
-    wp_store.
-    iModIntro.
-
-    iSplitL "Halive".
-    iNext.
-    iExists (n'+1).
-    iRight; auto.
-
-    iDestruct "Hlkinv" as (n1) "Hγ1●".
+    iDestruct (ghost_var_agree with "Hγ1● Hγ1◯") as %->.
     iMod (ghost_var_update γ1 (n+1) with "Hγ1● Hγ1◯") as "[Hγ1● Hγ1◯]".
+    wp_store.
     wp_pures.
     iApply "HPost".
-    iSplitL "Hγ1●".
-    iExists (n+1); auto.
-    iFrame; auto.
+    iSplitL "Hγ1● Halive"; auto.
+    iExists (n+1); auto. iFrame; auto.
   Qed.
 
   Lemma update_node_none_spec : ∀ (n: Z) γ1 node,
       {{{
-           node_lock_inv γ1
-          ∗ node_val_inv node true γ1
+           node_lock_inv node true γ1
           ∗ node_own_inv node n γ1
     }}}
       update_node #node
     {{{ RET #0;
-        node_lock_inv γ1
-        ∗ node_val_inv node true γ1
+        node_lock_inv node true γ1
         ∗ ∃ n, node_own_inv node n γ1
     }}}.
   Proof.
-    iIntros (n γ1 node Φ) "(Hlkinv & #Hnodeinv & Hγ1◯) HPost".
-    unfold node_val_inv.
-    unfold node_val_prop.
-    unfold update_node.
+    iIntros (n γ1 node Φ) "(Hlkinv & Hγ1◯) HPost".
     unfold node_lock_inv.
     unfold node_own_inv.
+    unfold update_node.
     wp_pures.
 
-    wp_bind ( ! #node )%E.
-    iInv "Hnodeinv" as ">Hinv".
-    iDestruct "Hinv" as (n') "[[H Halive] | [H Halive]]";
+    iDestruct "Hlkinv" as (n') "(Hγ1● & [[H Halive] | [H Halive]])";
     wp_load;
-    iDestruct "H" as %H; unfold not in H; simpl in H; try contradiction.
-    iModIntro.
-    iSplitL "Halive".
-    { iNext. unfold node_val_prop. iExists n'. iLeft. iSplitR "Halive"; auto. }
-
+    iDestruct "H" as %H; unfold not in H; destruct H; auto.
     wp_pures.
+    iDestruct (ghost_var_agree with "Hγ1● Hγ1◯") as %->.
     iApply "HPost".
-    iDestruct "Hlkinv" as (n1) "Hγ1●".
-    iSplitL "Hγ1●".
-    iExists (n1); auto.
-    iFrame; auto.
+    iSplitL "Hγ1● Halive"; auto.
+    iExists (n); auto. iFrame; auto.
   Qed.
 End proof.
